Otbn/Examples/Add32Linked.v
@@ -1,18 +1,141 @@
 Require Import Coq.Strings.String.
 Require Import Coq.Lists.List.
+Require Import Coq.micromega.Lia.
 Require Import Coq.ZArith.ZArith.
 Require Import coqutil.Byte.
 Require Import coqutil.Map.Interface.
 Require Import coqutil.Map.Properties.
 Require Import coqutil.Map.Separation.
+Require Import coqutil.Map.SeparationLogic.
 Require Import coqutil.Semantics.OmniSmallstepCombinators.
+Require Import coqutil.Tactics.Tactics.
 Require Import coqutil.Word.Interface.
 Require Import coqutil.Word.Properties.
+Require Import coqutil.Z.PushPullMod.
+Require Import Otbn.Examples.Add32.
+Require Import Otbn.Model.Clobbers.
 Require Import Otbn.Model.ISA.
 Require Import Otbn.Model.Linker.
+Require Import Otbn.Model.LinkerProperties.
 Require Import Otbn.Model.Semantics.
 Require Import Otbn.Model.SemanticsProperties.
 Require Import Otbn.Model.StraightlineStep.
+Require Import Otbn.Model.SubstLets.
 Import ListNotations.
 Import Semantics.Coercions.
 Local Open Scope Z_scope.
+
+(*** Test proving the *linked* version of a simple program. ***)
+
+(* NOTE: this is not a normal use-case! I just wanted to see if it would work. *)
+
+Section __.
+  Context {word32 : word.word 32} {word32_ok : word.ok word32}.
+  Context {word256 : word.word 256} {word256_ok : word.ok word256}.
+  Context {regfile : map.map reg word32} {regfile_ok : map.ok regfile}.
+  Context {wregfile : map.map wreg word256} {wregfile_ok : map.ok wregfile}.
+  Context {flagfile : map.map flag bool} {flagfile_ok : map.ok flagfile}.
+  Context {mem : map.map word32 byte} {mem_ok : map.ok mem}.
+  Add Ring wring32: (@word.ring_theory 32 word32 word32_ok).
+  Add Ring wring256: (@word.ring_theory 256 word256 word256_ok).
+
+  (* First, just try to prove the post-link program correct without
+     reusing any function specs or the linker proofs. *)
+  Lemma add_prog_correct_raw v dmem R :
+    (word32_at (word.of_Z 0) v * R)%sep dmem ->
+    eventually
+      (run1 (fetch:=fetch add_prog))
+      (fun st =>
+         match st with
+         | otbn_done _ dmem =>
+             (word32_at (word.of_Z 0) (word.of_Z 5) * R)%sep dmem
+         | _ => False
+         end)
+      (start_state dmem).
+  Proof.
+    cbv [add_prog start_state]; intros.
+    assert (word.unsigned (word:=word32) (word.of_Z 0) + 4 < DMEM_BYTES)
+      by (cbv [DMEM_BYTES]; rewrite word.unsigned_of_Z_0; lia).
+    repeat straightline_step.
+    eapply eventually_step_cps.
+    simplify_side_condition. 
+    repeat straightline_step.
+    eapply eventually_step_cps.
+    simplify_side_condition.
+    repeat straightline_step.
+    eapply eventually_ecall; [ reflexivity | ].
+    use_sep_assumption.
+    lazymatch goal with
+      |- Lift1Prop.iff1 (word_at ?ptr ?v1 * _)%sep (word_at ?ptr ?v2 * _)%sep =>
+        replace v2 with v1; [ ecancel | ]
+    end.
+    subst_lets.
+    cbv [addi_spec]. repeat destruct_one_match; try lia; [ ].
+    apply word.unsigned_inj.
+    rewrite !word.unsigned_add, !word.unsigned_of_Z_nowrap by lia.
+    cbv [word.wrap]. Z.push_pull_mod. reflexivity.
+  Qed.
+
+  (* Prove the pre-linked version of the program, using the function specification. *)
+  Lemma add_prog_correct_prelink regs wregs flags dmem (v : word32) R :
+    (word_at (word.of_Z 0) v * R)%sep dmem ->
+    exits
+      (fetch:=fetch_ctx [start_fn; add_fn])
+      "start"%string regs wregs flags dmem [] []
+      (word_at (width:=32) (word.of_Z 0) (word.of_Z 5) * R)%sep
+      (fun errs => False).
+  Proof.
+    cbv [exits start_fn start_state]; intros.
+    assert (word.unsigned (word:=word32) (word.of_Z 0) + 4 < DMEM_BYTES)
+      by (cbv [DMEM_BYTES]; rewrite word.unsigned_of_Z_0; lia).
+
+    repeat straightline_step.
+
+    eapply eventually_jump;
+      [ reflexivity | cbn [length]; lia | eapply add_correct; solve [eauto] | | ].
+    { intros.
+      rewrite fetch_ctx_weaken_cons_ne; [ eassumption | ].
+      eapply fetch_fn_disjoint; eauto; [ eapply fetch_ctx_singleton_iff; eauto | ].
+      cbv; intuition congruence. }
+
+    (* simplify hyps and combine register tracking post-jump *)
+    cbv beta. intros; subst.
+    repeat lazymatch goal with H : _ /\ _ |- _ => destruct H end.
+    track_registers_combine.
+
+    repeat straightline_step.
+
+    eapply eventually_ecall; ssplit; [ reflexivity .. | ].
+    use_sep_assumption.
+    lazymatch goal with
+      |- Lift1Prop.iff1 (word_at ?ptr ?v1 * _)%sep (word_at ?ptr ?v2 * _)%sep =>
+        replace v2 with v1; [ ecancel | ]
+    end.
+    subst_lets. cbv [addi_spec]. repeat destruct_one_match; try lia; [ ].
+    apply word.unsigned_inj.
+    rewrite !word.unsigned_add, !word.unsigned_of_Z_nowrap by lia.
+    cbv [word.wrap]. Z.push_pull_mod. reflexivity.
+  Qed.
+
+  (* Use the linker proofs and the pre-link proof to prove the post-link program *)
+  Lemma add_prog_correct_postlink dmem (v : word32) R :
+    (word_at (word.of_Z 0) v * R)%sep dmem ->
+    exits
+      (fetch:=fetch add_prog)
+      0%nat map.empty map.empty map.empty dmem [] []
+      (word_at (width:=32) (word.of_Z 0) (word.of_Z 5) * R)%sep
+      (fun errs => False).
+  Proof.
+    set (fns:=[start_fn; add_fn]). intros.
+    assert (link fns = inl add_prog) by reflexivity.
+    let x := eval vm_compute in (link_symbols [start_fn; add_fn]) in
+      match x with
+      | inl ?x =>
+          pose (syms:=x)
+      | _ => fail
+      end.
+    assert (link_symbols fns = inl syms) by reflexivity.
+    assert (find_global_offset fns "start"%string = Some 0%nat) by reflexivity.
+    eapply link_exits; eauto using add_prog_correct_prelink.
+  Qed.
+End __.
