Otbn/Examples/Mul32.v
@@ -1,0 +1,204 @@
+Require Import Coq.Strings.String.
+Require Import Coq.Lists.List.
+Require Import Coq.micromega.Lia.
+Require Import Coq.ZArith.ZArith.
+Require Import coqutil.Byte.
+Require Import coqutil.Map.Interface.
+Require Import coqutil.Map.Properties.
+Require Import coqutil.Map.Separation.
+Require Import coqutil.Map.SeparationLogic.
+Require Import coqutil.Semantics.OmniSmallstepCombinators.
+Require Import coqutil.Tactics.Tactics.
+Require Import coqutil.Word.Interface.
+Require Import coqutil.Word.Properties.
+Require Import coqutil.Z.PushPullMod.
+Require Import Otbn.Examples.Add32.
+Require Import Otbn.Model.Clobbers.
+Require Import Otbn.Model.ISA.
+Require Import Otbn.Model.Linker.
+Require Import Otbn.Model.Map.
+Require Import Otbn.Model.Semantics.
+Require Import Otbn.Model.SemanticsProperties.
+Require Import Otbn.Model.StraightlineStep.
+Require Import Otbn.Model.SubstLets.
+Require Import Otbn.Model.Zsimplify.
+Import ListNotations.
+Import Semantics.Coercions.
+Local Open Scope Z_scope.
+
+(*** Build 32-bit multiplication out of 32-bit addition. ***)
+
+(* Code reference:
+
+     mul:
+       addi   x2, x0, x0
+       beq    x4, x0, _mul_end
+       loop   x4, 2
+         jal    x1, add
+         addi   x2, x5, 0
+       _mul_end:
+       ret
+
+     add:
+       add  x5, x2, x3
+       ret
+*)
+
+Section __.
+  Context {word32 : word.word 32} {word32_ok : word.ok word32}.
+  Context {word256 : word.word 256} {word256_ok : word.ok word256}.
+  Context {regfile : map.map reg word32} {regfile_ok : map.ok regfile}.
+  Context {wregfile : map.map wreg word256} {wregfile_ok : map.ok wregfile}.
+  Context {flagfile : map.map flag bool} {flagfile_ok : map.ok flagfile}.
+  Context {mem : map.map word32 byte} {mem_ok : map.ok mem}.
+  Add Ring wring32: (@word.ring_theory 32 word32 word32_ok).
+  Add Ring wring256: (@word.ring_theory 256 word256 word256_ok).
+
+  (* Constructed in a way that avoids hardcoding the offset for the label. *)
+  Definition mul_fn : otbn_function :=
+    Eval cbn [List.app length] in (
+        let syms := map.empty in
+        let body : list insn :=
+          [ (Addi x2 x0 0 : insn);
+            (Beq x4 x0 "_mul_end" : insn);
+            (Loop x4 : insn);
+            (Jal x1 "add" : insn);
+            (Addi x2 x5 0 : insn);
+            (LoopEnd : insn)] in
+        let syms := map.put syms "_mul_end" (length body) in
+        let body := (body ++  [(Ret : insn)])%list in
+        ("mul", syms, body))%string.
+
+  
+  Lemma mul_correct :
+    forall regs wregs flags dmem cstack lstack a b,
+      map.get regs (gpreg x3) = Some a ->
+      map.get regs (gpreg x4) = Some b ->
+      (length cstack < 8)%nat ->
+      (length lstack < 8)%nat ->
+      returns
+        (fetch:=fetch_ctx [mul_fn; add_fn])
+        "mul"%string regs wregs flags dmem cstack lstack
+        (fun regs' wregs' flags' dmem' =>
+           map.get regs' (gpreg x2) = Some (word.mul a b)
+           /\ dmem' = dmem
+           /\ clobbers [] wregs wregs'
+           /\ clobbers [gpreg x2; gpreg x5] regs regs').
+  Proof.
+    cbv [mul_fn returns]. intros; subst. 
+    repeat straightline_step.
+ 
+    (* branch; use branch helper lemma *)
+    eapply eventually_beq.
+    { reflexivity. }
+    { simplify_side_condition; reflexivity. }
+    { simplify_side_condition; reflexivity. }
+    { (* case: b = 0, exit early *)
+      intros; subst. eapply eventually_ret; [ reflexivity | eassumption | ].
+      rewrite word.mul_0_r.
+      ssplit; try reflexivity; [ | | ].
+      { (* result value *)
+        mapsimpl; subst_lets. cbv [addi_spec].
+        destruct_one_match; try lia; [ ].
+        apply f_equal. ring. }
+      { assumption. }
+      { eapply clobbers_incl; eauto.
+        cbv [incl In]; tauto. } }
+    (* case: b <> 0, proceed *)
+    intros; subst.
+
+    pose proof (word.unsigned_range b).
+    assert (0 < word.unsigned b).
+    { lazymatch goal with H : b <> word.of_Z 0 |- _ =>
+                            apply word.unsigned_inj' in H end.
+      rewrite word.unsigned_of_Z_0 in *.
+      lia. }
+ 
+    (* loop; use loop invariant lemma *)
+    let loop_end_pc := find_loop_end in
+    eapply loop_invariant
+      with
+      (end_pc:=loop_end_pc)
+      (invariant :=
+         fun i regs' wregs' flags' dmem' =>
+           map.get regs' (gpreg x2) = Some (word.mul a (word.sub b (word.of_Z (Z.of_nat i))))
+           /\ map.get regs' (gpreg x3) = Some a
+           /\ map.get regs' (gpreg x4) = Some b
+           /\ dmem' = dmem
+           /\ clobbers [] flags flags'
+           /\ clobbers [] wregs wregs'
+           /\ clobbers [gpreg x2; gpreg x5] regs regs').
+    { reflexivity. }
+    { reflexivity. }
+    { simplify_side_condition; reflexivity. }
+    { apply Z2Nat.id; lia. }
+    { lia. }
+    { lia. }
+    { (* prove invariant holds at start *)
+      ssplit; simplify_side_condition; zsimplify; try reflexivity; [ | solve_clobbers ].
+      subst_lets. apply f_equal.
+      cbv [addi_spec]. destruct_one_match; try lia; [ ].
+      rewrite Z2Nat.id by lia.
+      rewrite word.of_Z_unsigned. ring. }
+    { (* invariant step; proceed through loop and prove invariant still holds *)
+      intros; subst. repeat lazymatch goal with H : _ /\ _ |- _ => destruct H end.
+
+      (* helper assertion that mul and add don't share symbols *)
+      assert (function_symbols_disjoint add_fn mul_fn).
+      { cbv [function_symbols_disjoint]; cbn [add_fn mul_fn fst snd].
+        ssplit; mapsimpl; try congruence; [ ].
+        cbv [map.disjoint]; intros *. rewrite map.get_empty; congruence. }
+
+      (* jump to "add" function *)
+      eapply eventually_jump.
+      { reflexivity. }
+      { lia. }
+      { apply add_correct; eauto. }
+      { intros.
+        rewrite fetch_ctx_weaken_cons_ne; [ eassumption | ].
+        eapply fetch_fn_disjoint; eauto; [ ].
+        eapply fetch_ctx_singleton_iff; eauto. }
+
+      (* post-jump; continue *)
+      cbv beta. intros; subst.
+      repeat lazymatch goal with H : _ /\ _ |- _ => destruct H end.
+      track_registers_combine.
+
+      repeat straightline_step.
+
+      (* end of loop; use loop-end helper lemma *)
+      eapply eventually_loop_end; [ reflexivity .. | ].
+      destruct_one_match.
+      { (* case: i = 0, loop ends *)
+        intros; subst. eapply eventually_done.
+        left. do 4 eexists; ssplit; [ .. | reflexivity ]; mapsimpl; [ ].
+        simplify_side_condition; subst_lets; zsimplify.
+        cbv [addi_spec]. destruct_one_match; try lia.
+        apply f_equal. ring. }
+      { (* case: 0 < i, loop continues *)
+        intros; subst. eapply eventually_done.
+        left. do 4 eexists; ssplit; [ .. | reflexivity ]; mapsimpl; [ ].
+        simplify_side_condition. subst_lets; zsimplify.
+        cbv [addi_spec]. destruct_one_match; try lia.
+        apply f_equal.
+        replace (word.of_Z (Z.of_nat (S (S i))))
+          with (word.add (word:=word32) (word.of_Z (Z.of_nat (S i))) (word.of_Z 1));
+          [ ring | ].
+        apply word.unsigned_inj.
+        rewrite !word.unsigned_add, !word.unsigned_of_Z_1 by lia.
+        rewrite !word.unsigned_of_Z_nowrap by lia.
+        cbv [word.wrap]; rewrite Z.mod_small by lia. lia. } }
+ 
+    (* invariant implies postcondition (i.e. post-loop code) *)
+    zsimplify. rewrite word.sub_0_r. intros.
+    repeat lazymatch goal with
+           | H : _ /\ _ |- _ => destruct H
+           | H : Some _ = Some _ |- _ => inversion H; clear H; subst
+           end.
+    simplify_side_condition.
+    repeat straightline_step.
+    intros; subst. eapply eventually_ret; [ reflexivity | eassumption | ].
+    ssplit; eauto.
+  Qed.
+
+End __.
