Otbn/Examples/RepeatAdd.v
@@ -1,0 +1,91 @@
+Require Import Coq.Strings.String.
+Require Import Coq.Lists.List.
+Require Import Coq.micromega.Lia.
+Require Import Coq.ZArith.ZArith.
+Require Import coqutil.Byte.
+Require Import coqutil.Map.Interface.
+Require Import coqutil.Map.Properties.
+Require Import coqutil.Map.Separation.
+Require Import coqutil.Map.SeparationLogic.
+Require Import coqutil.Semantics.OmniSmallstepCombinators.
+Require Import coqutil.Tactics.Tactics.
+Require Import coqutil.Word.Interface.
+Require Import coqutil.Word.Properties.
+Require Import coqutil.Z.PushPullMod.
+Require Import Otbn.Model.Clobbers.
+Require Import Otbn.Model.ISA.
+Require Import Otbn.Model.Linker.
+Require Import Otbn.Model.Map.
+Require Import Otbn.Model.Semantics.
+Require Import Otbn.Model.SemanticsProperties.
+Require Import Otbn.Model.StraightlineStep.
+Require Import Otbn.Model.SubstLets.
+Import ListNotations.
+Import Semantics.Coercions.
+Local Open Scope Z_scope.
+
+(*** Large code-generation process to test scaling. ***)
+
+Section __.
+  Context {word32 : word.word 32} {word32_ok : word.ok word32}.
+  Context {word256 : word.word 256} {word256_ok : word.ok word256}.
+  Context {regfile : map.map reg word32} {regfile_ok : map.ok regfile}.
+  Context {wregfile : map.map wreg word256} {wregfile_ok : map.ok wregfile}.
+  Context {flagfile : map.map flag bool} {flagfile_ok : map.ok flagfile}.
+  Context {mem : map.map word32 byte} {mem_ok : map.ok mem}.
+  Add Ring wring32: (@word.ring_theory 32 word32 word32_ok).
+  Add Ring wring256: (@word.ring_theory 256 word256 word256_ok).
+
+  (* Test scaling with a large codegen. *)
+  Definition repeat_add (n : nat) : otbn_function :=
+    (("add" ++ String.of_nat n)%string,
+      map.empty,
+      (Addi x2 x0 0 : insn) :: repeat (Add x2 x2 x3 : insn) n ++ [(Ret : insn)]).
+  Definition add100_fn : otbn_function := Eval vm_compute in (repeat_add 100).
+
+  (* helper lemma *)
+  Lemma mul_by_add_step x (a : word32) n :
+    0 < n ->
+    x = word.mul a (word.of_Z (n - 1)) ->
+    word.add x a = word.mul a (word.of_Z n).
+  Proof.
+    intros; subst. cbv [Z.sub].
+    rewrite word.ring_morph_add, word.ring_morph_opp.
+    ring.
+  Qed.
+
+  Lemma add100_correct :
+    forall regs wregs flags dmem cstack lstack a,
+      map.get regs (gpreg x3) = Some a ->
+      returns
+        (fetch:=fetch_ctx [add100_fn])
+        "add100"%string regs wregs flags dmem cstack lstack
+        (fun regs' wregs' flags' dmem' =>
+           map.get regs' (gpreg x2) = Some (word.mul a (word.of_Z 100))
+           /\ dmem' = dmem
+           /\ clobbers [] wregs wregs'
+           /\ clobbers [gpreg x2] regs regs').
+  Proof.
+    cbv [returns]; intros.
+    straightline_step.
+    Time do 10 straightline_step.
+    Time do 10 straightline_step.
+    Time do 10 straightline_step.
+    Time do 10 straightline_step.
+    Time do 10 straightline_step.
+    Time do 10 straightline_step.
+    Time do 10 straightline_step.
+    Time do 10 straightline_step.
+    Time do 10 straightline_step.
+    Time do 10 straightline_step. (* .57s *)
+
+    eapply eventually_ret; [ reflexivity | eassumption | ].
+    ssplit; try reflexivity; [ | solve_clobbers ..].
+    mapsimpl. apply (f_equal Some).
+    repeat (apply mul_by_add_step; [ lia | ];
+            cbn [Z.sub Z.add Z.opp Z.pos_sub Pos.pred_double]).
+    lazymatch goal with |- ?x = word.mul _ (word.of_Z 0) => subst x end.
+    cbv [addi_spec]. destruct_one_match; try lia; [ ].
+    ring.
+    Time Qed. (* 0.75s *)
+End __.
